Lean/Egg/Core/Gen/NestedSplits.lean
@@ -19,36 +19,31 @@ private def Congr.fresh (cgr : Congr) (mvars : MVars) (init : MVars.Subst := {})
 private structure Split where
   lhs     : Congr
   rhs     : Congr
+  srcDir  : Direction
   rwSrc   : Source
-  dir     : Direction
   rwProof : Expr
   rwRel   : Congr.Rel
 
 private def Split.type (split : Split) : MetaM Expr :=
-  match split.dir with
-  | .forward  => return .forallE .anonymous (← split.lhs.expr) (← split.rhs.expr) .default
-  | .backward => return .forallE .anonymous (← split.rhs.expr) (← split.lhs.expr) .default
+  return .forallE .anonymous (← split.lhs.expr) (← split.rhs.expr) .default
 
 private def Split.proof (split : Split) : MetaM Expr :=
-  match split.dir with
-  | .forward  => split.rwRel.mkMP  split.rwProof
-  | .backward => split.rwRel.mkMPR split.rwProof
+  split.rwRel.mkMP split.rwProof
 
 private def Split.src (split : Split) : Source :=
-  .nestedSplit split.rwSrc split.dir
+  .nestedSplit split.rwSrc split.srcDir
 
-private def Split.genRewrite (split : Split) (cfg : Config.Normalization) : MetaM Rewrite := do
-  let some rw ← Rewrite.from? (← split.proof) (← split.type) split.src cfg (normalize := false)
-    | throwError "egg: internal error: 'Egg.genSingleSplit' failed to construct rewrite"
-  return rw
+private def Split.genRewrites (split : Split) (cfg : Config.Normalization) : MetaM Rewrites := do
+  let some rws ← Rewrites.from? (← split.proof) (← split.type) split.src cfg (normalize := false)
+    | throwError "egg: internal error: 'Egg.Split.genRewrites failed to construct rewrite"
+  return rws
 
 private def genSplitsForRw (rw : Rewrite) (cfg : Config.Normalization) : MetaM Rewrites := do
   let some (lhs, rhs) ← rw.nested? | return #[]
   let mvars := rw.mvars.lhs.merge rw.mvars.rhs
   let (lhs, subst) ← lhs.fresh mvars
   let (rhs, _) ← rhs.fresh mvars (init := subst)
-  #[Direction.forward, .backward].mapM fun dir => do
-    Split.genRewrite { lhs, rhs, rwSrc := rw.src, dir, rwProof := rw.proof, rwRel := rw.rel } cfg
+  Split.genRewrites { lhs, rhs, srcDir := rw.dir, rwSrc := rw.src, rwProof := rw.proof, rwRel := rw.rel } cfg
 
 def genNestedSplits (targets : Rewrites) (cfg : Config.Normalization) : MetaM Rewrites := do
   targets.foldlM (init := #[]) fun acc rw => return acc ++ (← genSplitsForRw rw cfg)
