Lean/Egg/Core/Rewrite/Basic.lean
@@ -8,67 +8,36 @@ open Lean Meta
 namespace Egg
 
 -- Note: We don't create `Rewrite`s directly, but use `Rewrite.from?` instead.
-structure Rewrite extends Congr where
-  private mk ::
-  proof : Expr
-  src   : Source
+structure Rewrite extends Prerewrite where private mk ::
   conds : Array Rewrite.Condition
   mvars : Rewrite.MVars
-  -- TODO: Remove this
-  -- This is a means of fixing the set of directions for the rewrite manually.
-  private dirs? : Option Directions
+  src   : Source
+  dir   : Direction
   deriving Inhabited
+
+def Prerewrite.complete (pre : Prerewrite) (src : Source) (dir : Direction) : MetaM Rewrite := do
+  let pre ← pre.forDir dir
+  let mLhs  ← MVars.collect pre.lhs
+  let mRhs  ← MVars.collect pre.rhs
+  let conds ← collectConds pre.qvars mLhs mRhs
+  return { pre with conds, mvars := ⟨mLhs, mRhs⟩, src, dir }
+where
+  -- Note: It suffices to iterate over the qvars and the body mvars, as any mvars not appearing in
+  --       either of these must be the *type* of some mvar which does appear. But types can never
+  --       turn into conditions, so we don't need to consider them.
+  collectConds (qvars : MVarIdSet) (mLhs mRhs : MVars) : MetaM (Array Rewrite.Condition) := do
+    let mut mvars := qvars
+    mvars := mLhs.expr.fold (init := mvars) fun acc m _ => acc.insert m
+    mvars := mRhs.expr.fold (init := mvars) fun acc m _ => acc.insert m
+    mvars.toArray.filterMapM (Rewrite.Condition.from? · mLhs)
 
 namespace Rewrite
 
 def from?
-    (proof type : Expr) (src : Source) (cfg : Config.Normalization)
-    (normalize := true) (dir : Direction := .forward) : MetaM (Option Rewrite) := do
-  let mut some pre ← Prerewrite.from? proof type cfg normalize | return none
-  pre ← pre.forDir dir
-  let mLhs  ← MVars.collect pre.lhs
-  let mRhs  ← MVars.collect pre.rhs
-  let conds ← collectConds pre.qvars mLhs mRhs
-  return some { pre with src, conds, mvars.lhs := mLhs, mvars.rhs := mRhs, dirs? := none }
-where
-  collectConds (args : Array Expr) (mLhs mRhs : MVars) : MetaM (Array Rewrite.Condition) := do
-    let mut conds := #[]
-    -- Because of type class instance erasure, we need to make sure that all required type class
-    -- instances are synthesizable, so we add them as conditions to the rewrite. We only do this for
-    -- type class instances though which are erased as part of a type class instance term, because
-    -- "standalone" type class instances are represented by their erased term.
-    -- For example, we wouldn't add `?i` as a condition in `@Inhabited.default α ?i` as the erasure
-    -- of `?i` is precisely its type `Inhabited α`. In constrast, we would add `?j` as a condition
-    -- in `@HAdd.hAdd α α α (@instHAdd α j?)`, as the type of the entire type class instance term is
-    -- `HAdd α α α`, which doesn't match the type of `?j : Add α`.
-    for tcInstMVar in mLhs.nestedTcInsts.union mRhs.nestedTcInsts do
-      -- TODO: Collecting all this information seems a bit superfluos. Perhaps we should redefine
-      --       `Condition` (or split it into two types) as we only consider propositions and type
-      --       class instances anyway.
-      conds := conds.push {
-        kind  := .tcInst,
-        expr  := .mvar tcInstMVar,
-        type  := ← tcInstMVar.getType,
-        mvars := ← MVars.collect (← tcInstMVar.getType)
-      }
-    -- Even when erasure is active, we still do not consider the mvars contained in erased terms to
-    -- be conditions. Thus, we start by considering all mvars in the target as non-conditions and
-    -- take their type mvar closure. This closure will necessarily contain the mvars contained in
-    -- the types of erased terms, which therefore don't need to be added separately (as in,
-    -- contingent upon the erasure configuration).
-    let inTarget : MVarIdSet := mLhs.inTarget.union mRhs.inTarget
-    let mut noCond ← inTarget.typeMVarClosure
-    for arg in args.reverse do
-      if noCond.contains arg.mvarId! then continue
-      -- As we encode conditions as part of a rewrite's searcher its mvars also become
-      -- non-conditions. That's why we traverse the list of arguments above in reverse.
-      noCond := noCond.union (← MVarIdSet.typeMVarClosure {arg.mvarId!})
-      let ty ← arg.mvarId!.getType
-      let mvars ← MVars.collect ty
-      let some kind ← Condition.Kind.forType? ty
-        | throwError m!"Rewrite {src} requires condition of type '{ty}' which is neither a proof nor an instance."
-      conds := conds.push { kind, expr := arg, type := ty, mvars }
-    return conds
+    (dir : Direction) (proof type : Expr) (src : Source) (cfg : Config.Normalization)
+    (normalize := true) : MetaM <| Option Rewrite := do
+  let some pre ← Prerewrite.from? proof type cfg normalize | return none
+  pre.complete src dir
 
 -- Returns `none` if the given type is already ground.
 def mkGroundEq? (proof type : Expr) (src : Source) (cfg : Config.Normalization) (normalize := true) :
@@ -81,45 +50,59 @@ def mkGroundEq? (proof type : Expr) (src : Source) (cfg : Config.Normalization) 
   if type.hasLevelMVar then return none
   let cgr : Congr := { rel := .eq, lhs := type, rhs := .const ``True [] }
   let proof ← mkEqTrue proof
-  return some { cgr with proof, src, conds := #[], mvars.lhs := {}, mvars.rhs := {}, dirs? := none }
+  -- One direction suffices.
+  return some { cgr with qvars := ∅, proof, conds := #[], mvars := ⟨{}, {}⟩, src, dir := .forward }
 
--- If `disallowLoneMVar` is set, we prune directions where the pattern is just an mvar.
-def fixDirs (rw : Rewrite) (dirs : Directions) (disallowLoneMVar := false) : Rewrite := Id.run do
-  let mut d := dirs
-  if disallowLoneMVar then
-    if rw.lhs.isMVar then d := d.without .forward
-    if rw.rhs.isMVar then d := d.without .backward
-  { rw with dirs? := d }
+inductive Violation where
+  | rhsMVarInclusion (missing : MVarIdSet)
+  | lhsSingleMVar
+  | covering (missing : MVarIdSet)
+  | tcMVarInclusion
 
--- TODO: Have directions be a pair of values indicating whether the given direction is allowed,
---       and if not, then which restriction is not satisfied.
-def validDirs (rw : Rewrite) (conditionSubgoals : Bool) : Directions := Id.run do
-  if let some fixed := rw.dirs? then return fixed
-  let mut visibleExprLhs  := rw.mvars.lhs.visibleExpr
-  let mut visibleExprRhs  := rw.mvars.rhs.visibleExpr
-  let mut visibleLevelLhs := rw.mvars.lhs.visibleLevel
-  let mut visibleLevelRhs := rw.mvars.rhs.visibleLevel
-  if !conditionSubgoals then
-    -- MVars appearing in propositional conditions are going to be part of the rewrite's LHS, so
-    -- they can (and should be) ignored when computing valid directions.
-    -- TODO: How does visibility work in conditions?
-    let propCondExpr  : MVarIdSet  := rw.conds.filter (·.kind.isProof) |>.foldl (init := ∅) (·.union ·.mvars.visibleExpr)
-    let propCondLevel : LMVarIdSet := rw.conds.filter (·.kind.isProof) |>.foldl (init := ∅) (·.union ·.mvars.visibleLevel)
-    visibleExprLhs  := visibleExprLhs.filter  (!propCondExpr.contains ·)
-    visibleExprRhs  := visibleExprRhs.filter  (!propCondExpr.contains ·)
-    visibleLevelLhs := visibleLevelLhs.filter (!propCondLevel.contains ·)
-    visibleLevelRhs := visibleLevelRhs.filter (!propCondLevel.contains ·)
-  let exprDirs := Directions.satisfyingSuperset visibleExprLhs visibleExprRhs
-  let lvlDirs  := Directions.satisfyingSuperset visibleLevelLhs visibleLevelRhs
-  let mut dirs := exprDirs.meet lvlDirs
-  -- To avoid rewrites of the form "?m => ...", we disallow directions where the pattern is just an
-  -- mvar.
-  if rw.lhs.isMVar then dirs := dirs.without .forward
-  if rw.rhs.isMVar then dirs := dirs.without .backward
-  return dirs
+-- Note: To check `covering`, it suffices to check all qvars. The reason being that all vars are
+--       either in the theorem body, the qvars, or the types of the former. The variables in the
+--       body are covered by the LHS, as those in the RHS have to be a subset of that. The variables
+--       appearing only in types are covered by their "children", by type inference. Thus, we only
+--       have to check the qvars.
+--
+-- Note: In our procedure for checking `covering` we also assume that the construction for
+--       conditions is correct. As a result, all proof and type class instance variables are
+--       covered.
+--
+-- Note: When constructing `cov`, it's important to take the type mvar closure not only over
+--       `visible`, as this does not suffice when `subgoals = true`.
+--       Also note that taking the type mvar closure over the type class instances is ok, as we have
+--       `tcMVarInclusion` anyway.
+--
+-- TODO: Handle levels.
+def violation? (rw : Rewrite) (subgoals : Bool) : MetaM (Option Violation) := do
+  -- Checks for `lhsSingleMVar`.
+  if ← rw.lhs.isAmbientMVar <&&> ((return subgoals) <||> rw.conds.allM (·.type.isAmbientMVar)) then
+    return some .lhsSingleMVar
+  -- Checks for `rhsMVarInclusion`.
+  let visible :=
+    if subgoals then
+      rw.mvars.lhs.visibleExpr
+    else
+      rw.conds.foldl (init := rw.mvars.lhs.visibleExpr) fun vis cond =>
+        if cond.kind.isProof then vis.union cond.mvars.visibleExpr else vis
+  let missing := rw.mvars.rhs.visibleExpr.subtract visible
+  unless missing.isEmpty do return some (.rhsMVarInclusion missing)
+  -- Checks for `tcMVarInclusion`.
+  let tcVisible : MVarIdSet := rw.conds.foldl (init := ∅) fun vis cond =>
+    if cond.kind.isTcInst then vis.union cond.mvars.visibleExpr else vis
+  unless tcVisible.subset visible do return some .tcMVarInclusion
+  -- Checks for `covering`.
+  let mut cov ← rw.qvars.filterM fun m => Meta.isTCInstance (.mvar m) <||> Meta.isProof (.mvar m)
+  cov ← MVarIdSet.typeMVarClosure (cov.union visible)
+  let missing := rw.qvars.subtract cov
+  unless missing.isEmpty do return some (.covering missing)
+  return none
 
--- Returns the same rewrite but with its type and proof potentially flipped to match the given
--- direction.
+def isValid (rw : Rewrite) (subgoals : Bool) : MetaM Bool :=
+  return (← rw.violation? subgoals).isNone
+
+-- TODO: Flip the mvars and dir as well.
 def forDir (rw : Rewrite) : Direction → MetaM Rewrite
   | .forward  => return rw
   | .backward => return { rw with lhs := rw.rhs, rhs := rw.lhs, proof := ← rw.rel.mkSymm rw.proof }
@@ -133,6 +116,7 @@ def freshWithSubst (rw : Rewrite) (src : Source := rw.src) : MetaM (Rewrite × M
   let (mLhs, subst)  ← rw.mvars.lhs.fresh
   let (mRhs, subst)  ← rw.mvars.rhs.fresh (init := subst)
   let (conds, subst) ← freshConds (init := subst)
+  -- TODO: Refresh the qvars.
   -- Note: The `conds` already have `subst` applied. So If you have more substitution targets in the
   --       future, you might need to consider that.
   let rw' := { rw with
@@ -171,10 +155,11 @@ def instantiateMVars (rw : Rewrite) : MetaM Rewrite :=
   return { rw with
     lhs       := ← Lean.instantiateMVars rw.lhs
     rhs       := ← Lean.instantiateMVars rw.rhs
+    qvars     := ← rw.qvars.filterM fun m => return !(← m.isAssigned)
     proof     := ← Lean.instantiateMVars rw.proof
+    conds     := ← rw.conds.mapM (·.instantiateMVars)
     mvars.lhs := ← rw.mvars.lhs.removeAssigned
     mvars.rhs := ← rw.mvars.rhs.removeAssigned
-    conds     := ← rw.conds.mapM (·.instantiateMVars)
   }
 
 def pruneSynthesizableConditions (rw : Rewrite) : MetaM Rewrite := do
@@ -197,7 +182,16 @@ end Rewrite
 
 abbrev Rewrites := Array Rewrite
 
+namespace Rewrites
+
+-- Note: We are sharing mvars here. That should be ok, as we always create fresh mvars when *using*
+--       a rewrite anyway.
+def from? (proof type : Expr) (src : Source) (cfg : Config.Normalization) (normalize := true) :
+    MetaM <| Option Rewrites := do
+  let some pre ← Prerewrite.from? proof type cfg normalize | return none
+  return #[← pre.complete src .forward, ← pre.complete src .backward]
+
 -- TODO: This is unnecessarilly inefficient during proof reconstruction. At some point we may want
 --       to redefine `Rewrites` using a better suited data structure like `HashMap Source Rewrite`.
-def Rewrites.find? (rws : Rewrites) (src : Source) : Option Rewrite :=
+def find? (rws : Rewrites) (src : Source) : Option Rewrite :=
   Array.find? (·.src == src) rws
