Lean/Egg/Lean.lean
@@ -48,6 +48,10 @@ end Std.HashMap
 
 namespace Lean
 
+def Expr.isAmbientMVar (e : Expr) : MetaM Bool := do
+  let .mvar m := e | return false
+  return !(← m.isAssignable)
+
 /-
 This terminates because the types of mvars aren't simply mvars again:
 ```
