Lean/Egg/Tests/Condition Kind.lean
@@ -1,6 +1,9 @@
 import Egg
 
-/-- error: Rewrite #0 requires condition of type 'Nat' which is neither a proof nor an instance. -/
+-- This test should fail, because both directions of `h` are invalid, because the `Nat` argument is
+-- not covered, because it can't be a condition, because it's neither a proof nor an instance.
+
+/-- error: egg failed to prove the goal (saturated) -/
 #guard_msgs in
 example (h : Nat → 0 = 1) : 0 = 1 := by
   egg [h]
