Lean/Egg/Tests/MVars Properties.lean
@@ -11,7 +11,7 @@ set_option trace.egg.rewrites true
 info: [egg.rewrites] Rewrites
   [egg.rewrites] Intros (0)
   [egg.rewrites] Basic (1)
-    [egg.rewrites] #0(∅): h
+    [egg.rewrites] #0(⇒): h
       [egg.rewrites] ?x = ?x
       [egg.rewrites] LHS MVars
           [?x: [unconditionallyVisible]]
@@ -22,7 +22,12 @@ info: [egg.rewrites] Rewrites
   [egg.rewrites] Derived (0)
   [egg.rewrites] Structure Projections (0)
   [egg.rewrites] Definitional
-  [egg.rewrites] Pruned (0)
+  [egg.rewrites] Pruned (1)
+    [egg.rewrites] #0(⇐) by #0
+      [egg.rewrites] ?x = ?x
+      [egg.rewrites] LHS MVars
+          [?x: [unconditionallyVisible]]
+      [egg.rewrites] RHS MVars [?x: [unconditionallyVisible]]
 -/
 #guard_msgs(info) in
 example (h : ∀ x : Nat, x = x) : true = true := by
@@ -31,13 +36,19 @@ example (h : ∀ x : Nat, x = x) : true = true := by
 /--
 info: [egg.rewrites] Rewrites
   [egg.rewrites] Intros (0)
-  [egg.rewrites] Basic (1)
+  [egg.rewrites] Basic (2)
     [egg.rewrites] #0(⇒): h
       [egg.rewrites] f ?x = ?x
       [egg.rewrites] LHS MVars
-          [?x: [unconditionallyVisible], ?α: [unconditionallyVisible]]
+          [?α: [unconditionallyVisible], ?x: [unconditionallyVisible]]
       [egg.rewrites] RHS MVars
           [?x: [unconditionallyVisible]]
+    [egg.rewrites] #0(⇐)(❌rhsMVarInclusion: [?α]): h
+      [egg.rewrites] ?x = f ?x
+      [egg.rewrites] LHS MVars
+          [?x: [unconditionallyVisible]]
+      [egg.rewrites] RHS MVars
+          [?α: [unconditionallyVisible], ?x: [unconditionallyVisible]]
   [egg.rewrites] Tagged (0)
   [egg.rewrites] Builtin (0)
   [egg.rewrites] Derived (0)
@@ -52,15 +63,23 @@ example (f : {α : Type} → α → α) (h : ∀ α (x : α), f x = x) : true = 
 /--
 info: [egg.rewrites] Rewrites
   [egg.rewrites] Intros (0)
-  [egg.rewrites] Basic (1)
+  [egg.rewrites] Basic (2)
     [egg.rewrites] #0(⇒): h
       [egg.rewrites] ?x + ?x = ?x
       [egg.rewrites] Conditions
         [egg.rewrites] Add α
       [egg.rewrites] LHS MVars
-          [?x: [unconditionallyVisible], ?inst✝: [inTcInstTerm, isTcInst]]
+          [?inst✝: [inTcInstTerm, isTcInst], ?x: [unconditionallyVisible]]
       [egg.rewrites] RHS MVars
           [?x: [unconditionallyVisible]]
+    [egg.rewrites] #0(⇐): h
+      [egg.rewrites] ?x = ?x + ?x
+      [egg.rewrites] Conditions
+        [egg.rewrites] Add α
+      [egg.rewrites] LHS MVars
+          [?x: [unconditionallyVisible]]
+      [egg.rewrites] RHS MVars
+          [?inst✝: [inTcInstTerm, isTcInst], ?x: [unconditionallyVisible]]
   [egg.rewrites] Tagged (0)
   [egg.rewrites] Builtin (0)
   [egg.rewrites] Derived (0)
@@ -75,13 +94,19 @@ example (h : ∀ [Add α] (x : α), x + x = x) : true = true := by
 /--
 info: [egg.rewrites] Rewrites
   [egg.rewrites] Intros (0)
-  [egg.rewrites] Basic (1)
+  [egg.rewrites] Basic (2)
     [egg.rewrites] #0(⇒): h
       [egg.rewrites] f ?n ⋯ = ?n
       [egg.rewrites] LHS MVars
           [?n: [inErasedProof, inProofTerm, unconditionallyVisible]]
       [egg.rewrites] RHS MVars
           [?n: [unconditionallyVisible]]
+    [egg.rewrites] #0(⇐): h
+      [egg.rewrites] ?n = f ?n ⋯
+      [egg.rewrites] LHS MVars
+          [?n: [unconditionallyVisible]]
+      [egg.rewrites] RHS MVars
+          [?n: [inErasedProof, inProofTerm, unconditionallyVisible]]
   [egg.rewrites] Tagged (0)
   [egg.rewrites] Builtin (0)
   [egg.rewrites] Derived (0)
