Lean/Egg/Tests/Subgoals.lean
@@ -22,14 +22,13 @@ h : p → q → a = b
 example (a : Nat) (p q : Prop) (h : p → q → a = b) : a = b := by
   egg [h]
 
-
 /--
 error: unsolved goals
 h : ∀ (m : Nat), m = 0 → 1 = 2
 ⊢ Nat
 
 h : ∀ (m : Nat), m = 0 → 1 = 2
-⊢ ?m.781 = 0
+⊢ ?m.1274 = 0
 -/
 #guard_msgs in
 example (h : ∀ m, m = 0 → 1 = 2) : 1 = 2 := by
